A new way to get from eval' to eval
Basically a simple type system based on a syntactic check that all of
the constructor applications are to existing constructors with the right
number of arguments.  Also, pattern matches are very restricted and must
not contain any nested patterns, and each constructor pattern must have
a constructor from the same type as the other constructors in the match.

Proved for evaluate' and evaluate_dec', but not for evaluate_decs' or
evaluate_top'.

metatheory/bigBigEquivScript.sml
@@ -1,10 +1,37 @@
 open preamble
 open SemanticPrimitivesTheory AltBigStepTheory BigStepTheory TypeSystemTheory;
 open bigSmallEquivTheory determTheory untypedSafetyTheory;
-open typeSoundTheory;
+open typeSysPropsTheory typeSoundTheory;
 open terminationTheory bigClockTheory;
 
 val _ = new_theory "bigBigEquiv"
+
+val big_exp_determ' = Q.store_thm ("big_exp_determ'",
+`(∀s env e r1.
+   evaluate' s env e r1 ⇒
+   ∀r2. evaluate' s env e r2 ⇒
+   (r1 = r2)) ∧
+ (∀s env es r1.
+   evaluate_list' s env es r1 ⇒
+   ∀r2. evaluate_list' s env es r2 ⇒
+   (r1 = r2)) ∧
+ (∀s env v pes r1.
+   evaluate_match' s env v pes r1 ⇒
+   ∀r2. evaluate_match' s env v pes r2 ⇒
+   (r1 = r2))`,
+HO_MATCH_MP_TAC evaluate'_ind >>
+rw [] >>
+pop_assum (ASSUME_TAC o SIMP_RULE (srw_ss ()) [Once evaluate'_cases]) >>
+fs [] >>
+rw [] >>
+fs [] >>
+res_tac >>
+fs [] >>
+rw [] >>
+res_tac >>
+fs [] >>
+rw [] >> 
+metis_tac []);
 
 val pmatch_pmatch' = Q.prove (
 `(!(cenv : envC)  (s:store) p v env. (pmatch cenv s p v env ≠ Match_type_error) ⇒
@@ -198,21 +225,22 @@ val eval_prog'_to_eval_prog_thm = Q.store_thm ("eval_prog'_to_eval_prog_thm",
 metis_tac [eval_prog'_to_eval_prog, prog_type_soundness, untyped_safety_prog, prog_determ, PAIR_EQ]);
 *)
 
-val atomic_pat_def = Define `
-(atomic_pat (Pvar x) = T) ∧
-(atomic_pat (Plit x) = T)`;
+val var_pat_def = Define `
+(var_pat (Pvar x) = T) ∧
+(var_pat _ = F)`;
 
 val check_ctors_p_def = Define `
-(check_ctors_p cenv t (Pvar x) = T) ∧
-(check_ctors_p cenv t (Plit l) = T) ∧
-(check_ctors_p cenv t (Pcon cn ps) =
+(check_ctors_p cenv NONE (Pvar x) = T) ∧
+(check_ctors_p cenv NONE (Plit l) = T) ∧
+(check_ctors_p cenv (SOME t) (Pcon cn ps) =
   case lookup cn cenv of
      | NONE => F
      | SOME (len, tn) =>
-         (t = SOME tn) ∧
+         (t = tn) ∧
          (len = LENGTH ps) ∧
-         EVERY atomic_pat ps) ∧
-(check_ctors_p cenv t (Pref p) = atomic_pat p)`;
+         EVERY var_pat ps) ∧
+(check_ctors_p cenv NONE (Pref p) = var_pat p) ∧
+(check_ctors_p cenv _ _ = F)`;
 
 val get_pat_type_def = Define `
 (get_pat_type cenv (Pvar x) = NONE) ∧
@@ -222,6 +250,24 @@ val get_pat_type_def = Define `
   case lookup cn cenv of
      | NONE => NONE
      | SOME (len, tn) => SOME tn)`;
+
+val get_pat_type_thm = Q.prove (
+`!cenv p1 p2.
+  check_ctors_p cenv (get_pat_type cenv p1) p2
+  ⇒
+  (get_pat_type cenv p1 = get_pat_type cenv p2)`,
+cases_on `p1` >>
+rw [get_pat_type_def, check_ctors_p_def] >>
+cases_on `p2` >>
+fs [get_pat_type_def, check_ctors_p_def] >>
+cases_on `lookup i cenv` >>
+fs [] >>
+TRY (PairCases_on `x`) >>
+fs [check_ctors_p_def] >>
+cases_on `lookup i' cenv` >>
+fs [] >>
+PairCases_on `x` >>
+fs []);
 
 val check_ctors_def = tDefine "check_ctors" `
 (check_ctors (cenv:envC) (Raise e) = T) ∧
@@ -285,144 +331,504 @@ srw_tac [ARITH_ss] [AstTheory.exp_size_def, v_size_def] >>
 res_tac >>
 decide_tac);
 
-(*
-val eval_check_ctors_pres = Q.prove (
-`(∀ck (menv : envM) (cenv : envC) s env e r.
-   evaluate ck menv cenv s env e r ⇒
-   !count s1 r1 v.
-     (r = ((count,s1), Rval v)) ⇒
-     check_ctors_v cenv v) ∧
- (∀ck (menv : envM) (cenv : envC) s env es r.
-   evaluate_list ck menv cenv s env es r ⇒
-   !count s1 r1 v.
-     (r = ((count,s1), Rval v)) ⇒
-     EVERY (check_ctors_v cenv) v) ∧
- (∀ck (menv : envM) (cenv : envC) s env v pes r.
-   evaluate_match ck menv cenv s env v pes r ⇒
-   !count s1 r1 v.
-     (r = ((count,s1), Rval v)) ⇒
-     check_ctors_v cenv v)`,
+val check_var_pat = Q.prove (
+`(!p. var_pat p ⇒ check_ctors_p cenv NONE p) ∧
+ (!ps. EVERY var_pat ps ⇒ EVERY (check_ctors_p cenv NONE) ps)`,
+Induct >>
+rw [var_pat_def, check_ctors_p_def] >>
+metis_tac []);
 
-ho_match_mp_tac evaluate_ind >>
-rw [check_ctors_v_def] >|
-[fs [do_con_check_def] >>
-     every_case_tac >>
-     rw []
-     *)
+val eval_ctor_inv_def = Define `
+eval_ctor_inv cenv s env =
+  (EVERY (check_ctors_v cenv) s ∧
+   EVERY (\(x,v). check_ctors_v cenv v) env)`;
 
-     (*
-val pmatch'_pmatch2 = Q.prove (
-`(!(cenv : envC) (s:store) p v env t. 
-   EVERY (check_ctors_v cenv) s ∧ check_ctors_p cenv t p ∧ check_ctors_v cenv v ⇒
-   (pmatch' s p v env = pmatch cenv s p v env)) ∧
- (!(cenv : envC) (s:store) ps vs env env' t. 
-    EVERY (check_ctors_v cenv) s ∧ EVERY (check_ctors_p cenv t) ps ∧ EVERY (check_ctors_v cenv) vs ⇒
-   (pmatch_list' s ps vs env = pmatch_list cenv s ps vs env))`,
-cheat)
-ho_match_mp_tac pmatch_ind >>
-rw [pmatch_def, pmatch'_def, check_ctors_p_def, check_ctors_v_def] >|
-[Cases_on `lookup n cenv` >>
-     fs [do_con_check_def] >>
-     Cases_on `x` >>
-     fs [] >>
-     metis_tac [],
- Cases_on `lookup n cenv` >>
-     fs [do_con_check_def] >>
-     Cases_on `x` >>
-     fs [] >>
-     metis_tac [],
- Cases_on `lookup n cenv` >>
-     fs [do_con_check_def] >>
-     Cases_on `x` >>
-     fs [] >>
-     every_case_tac >>
-     fs [] >>
-     rw [] >>
-     all_tac,
- every_case_tac >>
-     fs [store_lookup_def, EVERY_EL] >>
-     metis_tac [],
- every_case_tac >>
-     fs []]);
+val eval_ctor_inv_bind_env = Q.prove (
+`!cenv s x v env.
+  eval_ctor_inv cenv s (bind x v env) =
+  (check_ctors_v cenv v ∧ eval_ctor_inv cenv s env)`,
+rw [eval_ctor_inv_def, LibTheory.bind_def, eval_ctor_inv_def] >>
+metis_tac []);
 
-val unfinished = all_tac;
-val eval'_to_eval2 = Q.prove (
-`(!s env e r. evaluate' s env e r ⇒
-   !menv cenv count s1 r1. (r = (s1,r1)) ∧ check_ctors cenv e ⇒
-   evaluate F menv cenv (count,s) env e ((count,s1),r1)) ∧
- (!s env es r. evaluate_list' s env es r ⇒
-   !menv cenv count s1 r1. (r = (s1,r1)) ∧ EVERY (check_ctors cenv) es ⇒
-   evaluate_list F menv cenv (count,s) env es ((count,s1),r1)) ∧
- (!s env v pes r. evaluate_match' s env v pes r ⇒
-   !menv (cenv:envC) count s1 r1. (r = (s1,r1)) ∧
-   EVERY (\(p,e). check_ctors_p cenv (get_pat_type cenv (FST (HD pes))) p ∧ check_ctors cenv e) pes ⇒
-   evaluate_match F menv cenv (count,s) env v pes ((count,s1),r1))`,
+val eval_ctor_inv_lookup = Q.prove (
+`!cenv s env n v.
+  eval_ctor_inv cenv s env ∧
+  (lookup n env = SOME v) ⇒
+  check_ctors_v cenv v`,
+rw [eval_ctor_inv_def, LibTheory.bind_def, eval_ctor_inv_def] >>
+imp_res_tac lookup_in >>
+fs [GSYM PEXISTS_THM, GSYM PFORALL_THM, LAMBDA_PROD, MEM_MAP, EVERY_MEM] >>
+rw [] >>
+metis_tac []);
 
-ho_match_mp_tac evaluate'_ind >>
+val eval_ctor_inv_do_uapp = Q.prove (
+`!s1 uop v1 s2 v2.
+  (do_uapp s1 uop v1 = SOME (s2, v2)) ∧
+  eval_ctor_inv cenv s1 env ∧
+  check_ctors_v cenv v1
+  ⇒
+  check_ctors_v cenv v2 ∧
+  eval_ctor_inv cenv s2 env`,
+rw [do_uapp_def, eval_ctor_inv_def, check_ctors_v_def] >>
+cases_on `uop` >>
+cases_on `v1` >>
+fs [check_ctors_v_def, LET_THM, store_alloc_def] >>
+rw [check_ctors_v_def] >>
+cases_on `store_lookup n s1` >>
+fs [store_lookup_def, EVERY_MEM, LAMBDA_PROD, GSYM PFORALL_THM] >>
+metis_tac [MEM_EL]);
+
+val eval_ctor_build_rec_env = Q.prove (
+`!cenv s funs1 funs2 cl_env add_to_env.
+  eval_ctor_inv cenv s add_to_env ∧
+  eval_ctor_inv cenv s cl_env ∧
+  EVERY (λ(f,x,e). check_ctors cenv e) funs1
+  ⇒
+  eval_ctor_inv cenv s ( FOLDR (λ(f,x,e) env'. bind f (Recclosure cl_env funs1 f) env') add_to_env funs2)`,
+induct_on `funs2` >>
+rw [] >>
+PairCases_on `h` >>
+fs [eval_ctor_inv_bind_env, build_rec_env_def, check_ctors_v_def] >>
+fs [eval_ctor_inv_def]);
+
+val eval_ctor_inv_do_app = Q.prove (
+`!s1 env1 op v1 v2 s2 env2 e.
+  (do_app s1 env1 op v1 v2 = SOME (s2,env2,e)) ∧
+  eval_ctor_inv cenv s1 env1 ∧
+  check_ctors_v cenv v1 ∧
+  check_ctors_v cenv v2
+  ⇒
+  check_ctors cenv e ∧
+  eval_ctor_inv cenv s2 env2`,
+rw [do_app_cases] >>
 rw [check_ctors_def] >>
+fs [check_ctors_v_def, eval_ctor_inv_bind_env] >|
+[fs [eval_ctor_inv_def],
+ induct_on `funs` >>
+     rw [Once find_recfun_def] >>
+     PairCases_on `h` >>
+     fs [] >>
+     cases_on `h0 = n'` >>
+     fs [] >>
+     metis_tac [],
+ rw [build_rec_env_def] >>
+     match_mp_tac eval_ctor_build_rec_env >>
+     fs [eval_ctor_inv_def],
+ fs [store_assign_def, eval_ctor_inv_def] >>
+     fs [EVERY_EL] >>
+     rw [EL_LUPDATE]]);
+
+val eval_ctor_inv_do_log = Q.prove (
+`!op v e1 e2.
+  (do_log op v e1 = SOME e2) ∧
+  check_ctors_v cenv v ∧
+  check_ctors cenv e1 
+  ⇒
+  check_ctors cenv e2`, 
+rw [do_log_def] >>
+cases_on `v` >>
+fs [] >>
+cases_on `l` >>
+fs [] >>
+cases_on `b` >>
+fs [] >>
+cases_on `op` >>
+fs [] >>
+rw [] >>
+fs [check_ctors_def]);
+
+val eval_ctor_inv_do_if = Q.prove (
+`!v e1 e2 e3.
+  (do_if v e1 e2 = SOME e3) ∧
+  check_ctors_v cenv v ∧
+  check_ctors cenv e1 ∧
+  check_ctors cenv e2 
+  ⇒
+  check_ctors cenv e3`, 
+rw [do_if_def] >>
+metis_tac []);
+
+val check_ctors_result_def = Define `
+(check_ctors_result cenv (Rval v) = check_ctors_v cenv v) ∧
+(check_ctors_result cenv _ = T)`;
+
+val check_ctors_result2_def = Define `
+(check_ctors_result2 cenv n (Rval vs) = ((LENGTH vs = n) ∧ EVERY (check_ctors_v cenv) vs)) ∧
+(check_ctors_result2 cenv n _ = T)`;
+
+val check_ctors_match_result_def = Define `
+(check_ctors_match_result cenv s (Match env) = 
+  eval_ctor_inv cenv s env) ∧
+(check_ctors_match_result cenv s _ = T)`;
+
+val get_val_type_def = Define `
+(get_val_type cenv (Conv cn vs) = 
+  case lookup cn cenv of
+     | NONE => NONE
+     | SOME (len, tn) => SOME tn) ∧
+(get_val_type cenv _ = NONE)`;
+
+val pmatch'_pmatch2_lem = Q.prove (
+`!ps vs env.
+  (LENGTH ps = LENGTH vs) ∧
+  EVERY var_pat ps ∧
+  EVERY (check_ctors_v cenv) vs ∧
+  eval_ctor_inv cenv s env
+  ⇒
+  (pmatch_list' s ps vs env = pmatch_list cenv s ps vs env) ∧
+  check_ctors_match_result cenv s (pmatch_list cenv s ps vs env)`,
+Induct >>
+rw [] >>
+cases_on `vs` >>
+fs [pmatch_def, pmatch'_def, check_ctors_match_result_def, var_pat_def] >>
+cases_on `h` >>
+fs [pmatch_def, pmatch'_def, check_ctors_match_result_def, var_pat_def] >>
+metis_tac [eval_ctor_inv_bind_env]);
+
+val pmatch'_pmatch2 = Q.prove (
+`!(cenv : envC) (s:store) p v env (menv : envM) t. 
+  eval_ctor_inv cenv s env ∧ 
+  check_ctors_p cenv t p ∧ 
+  check_ctors_v cenv v 
+  ⇒
+  check_ctors_match_result cenv s (pmatch cenv s p v env) ∧
+  ((pmatch' s p v env = pmatch cenv s p v env) ∨
+   (?t1 t2. 
+      pmatch' s p v env = No_match ∧
+      pmatch cenv s p v env = Match_type_error ∧
+      (get_pat_type cenv p = SOME t1) ∧ 
+      (get_val_type cenv v = SOME t2) ∧ 
+      t1 ≠ t2))`,
+cases_on `p` >>
+cases_on `v` >>
+cases_on `t` >>
+fs [pmatch_def, pmatch'_def, check_ctors_p_def, check_ctors_v_def, eval_ctor_inv_bind_env,
+    check_ctors_match_result_def, get_pat_type_def, get_val_type_def] >-
+rw [check_ctors_match_result_def] >|
+[NTAC 5 strip_tac >>
+     Cases_on `lookup i cenv` >>
+     fs [] >>
+     Cases_on `x'` >>
+     fs [] >>
+     Cases_on `lookup i' cenv` >>
+     fs [do_con_check_def, check_ctors_p_def] >>
+     Cases_on `x'` >>
+     fs [check_ctors_p_def, check_ctors_match_result_def] >>
+     rw [check_ctors_match_result_def] >>
+     fs [] >>
+     metis_tac [pmatch'_pmatch2_lem],
+ NTAC 5 STRIP_TAC >>
+     every_case_tac >>
+     fs [store_lookup_def, EVERY_EL] >>
+     fs [check_ctors_p_def, EVERY_EL, eval_ctor_inv_def, check_ctors_match_result_def] >>
+     cases_on `p'` >>
+     fs [var_pat_def, pmatch_def, pmatch'_def, check_ctors_match_result_def,
+         eval_ctor_inv_bind_env] >>
+     fs [eval_ctor_inv_def, EVERY_EL] >>
+     metis_tac []]);
+
+val pmatch'_wrong_type = Q.prove (
+`!cenv p v t1 t2 p'.
+  (get_pat_type cenv p = SOME t1) ∧
+  (get_val_type cenv v = SOME t2) ∧
+  t1 ≠ t2 ∧
+  check_ctors_p cenv (get_pat_type cenv p) p'
+  ⇒
+  pmatch' s p' v env = No_match`,
+cases_on `p` >>
+cases_on `v` >>
+rw [get_pat_type_def, get_val_type_def] >>
+every_case_tac >>
+fs [] >>
+cases_on `p'` >>
+fs [check_ctors_p_def, pmatch'_def, get_pat_type_def, get_val_type_def] >>
+rw [] >>
+cases_on `lookup i' cenv` >>
+fs []);
+
+val eval'_to_eval2_lem = Q.prove (
+`!pes cenv p v t1 t2 s env count.
+  (get_pat_type cenv p = SOME t1) ∧
+  (get_val_type cenv v = SOME t2) ∧
+  t1 ≠ t2 ∧
+  (∀e. MEM e pes ⇒
+        (λ(p',e').
+           check_ctors_p cenv (get_pat_type cenv p) p' ∧
+           check_ctors cenv e') e)
+  ⇒
+  evaluate_match' s env v pes (s, Rerr (Rraise Bind_error)) ∨
+  evaluate_match' s env v pes (s, Rerr Rtype_error)`,
+induct_on `pes` >>
+rw [] >>
+ONCE_REWRITE_TAC [evaluate_cases, evaluate'_cases] >>
+rw [] >>
+`(λ(p',e'). check_ctors_p cenv (get_pat_type cenv p) p' ∧ check_ctors cenv e') h`
+        by metis_tac [] >>
+PairCases_on `h` >>
+fs [] >>
+cases_on `ALL_DISTINCT (pat_bindings h0 [])` >>
+fs [] >>
+`pmatch' s h0 v env = No_match` by metis_tac [pmatch'_wrong_type] >>
+rw [] >>
+`evaluate_match' s env v pes (s,Rerr (Rraise Bind_error)) ∨
+ evaluate_match' s env v pes (s,Rerr Rtype_error)`
+         by metis_tac [] >>
+rw [] >>
+metis_tac []);
+
+val eval'_to_eval_simple_pat = Q.store_thm ("eval'_to_eval_simple_pat",
+`(!s env e r. evaluate' s env e r ⇒
+   !menv cenv count s1 r1. (r = (s1,r1)) ∧ r1 ≠ Rerr (Rraise Bind_error) ∧ check_ctors cenv e ∧
+      eval_ctor_inv cenv s env ⇒
+      eval_ctor_inv cenv s1 env ∧
+      check_ctors_result cenv r1 ∧
+      evaluate F menv cenv (count,s) env e ((count,s1),r1)) ∧
+ (!s env es r. evaluate_list' s env es r ⇒
+   !menv cenv count s1 r1. (r = (s1,r1)) ∧ r1 ≠ Rerr (Rraise Bind_error) ∧ EVERY (check_ctors cenv) es ∧
+      eval_ctor_inv cenv s env ⇒
+      eval_ctor_inv cenv s1 env ∧
+      check_ctors_result2 cenv (LENGTH es) r1 ∧
+      evaluate_list F menv cenv (count,s) env es ((count,s1),r1)) ∧
+ (!s env v pes r. evaluate_match' s env v pes r ⇒
+   !menv (cenv:envC) count s1 r1. (r = (s1,r1)) ∧ r1 ≠ Rerr (Rraise Bind_error) ∧
+      check_ctors_v cenv v ∧
+      EVERY (\(p,e). check_ctors_p cenv (get_pat_type cenv (FST (HD pes))) p ∧ check_ctors cenv e) pes ∧
+      eval_ctor_inv cenv s env ⇒
+      eval_ctor_inv cenv s1 env ∧
+      check_ctors_result cenv r1 ∧
+      evaluate_match F menv cenv (count,s) env v pes ((count,s1),r1))`,
+ho_match_mp_tac evaluate'_strongind >>
+REPEAT CONJ_TAC >>
+REPEAT GEN_TAC >>
+REPEAT DISCH_TAC >>
+REPEAT GEN_TAC >>
+STRIP_TAC >>
 SIMP_TAC (srw_ss()) [Once evaluate_cases] >>
 fs [] >>
-fs [lookup_var_id_def, EVERY_MEM] >|
-[metis_tac [],
- metis_tac [],
- metis_tac [],
-(* `check_ctors cenv e''`
-            by (fs [do_app_cases] >>
-                rw [check_ctors_def])
-                *)
- unfinished,
- metis_tac [],
- metis_tac [],
- `check_ctors cenv e'`
-            by (fs [do_log_def] >>
-                rw [] >>
-                cases_on `v` >>
-                fs [] >>
-                cases_on `l` >>
-                fs [] >>
-                every_case_tac >>
-                rw [check_ctors_def]) >>
+fs [lookup_var_id_def, EVERY_MEM, check_ctors_result_def, check_ctors_v_def, check_ctors_def] >|
+[metis_tac [check_ctors_result_def, check_ctors_v_def],
+ metis_tac [check_ctors_result_def, check_ctors_v_def],
+ metis_tac [check_ctors_result_def, check_ctors_v_def],
+ metis_tac [check_ctors_result_def, check_ctors_v_def],
+ metis_tac [check_ctors_result_def, check_ctors_v_def],
+ metis_tac [check_ctors_result_def, check_ctors_v_def, eval_ctor_inv_bind_env],
+ metis_tac [check_ctors_result_def, check_ctors_v_def],
+ metis_tac [check_ctors_result_def, check_ctors_v_def],
+ metis_tac [check_ctors_result_def, check_ctors_v_def],
+ res_tac >>
+     fs [do_con_check_def, check_ctors_result_def, check_ctors_v_def, check_ctors_result2_def] >>
+     rw [check_ctors_result_def, check_ctors_v_def, do_con_check_def] >>
+     every_case_tac >>
+     fs [] >>
      metis_tac [],
- metis_tac [],
- `check_ctors cenv e'`
-            by (fs [do_if_def] >>
-                rw [] >>
-                every_case_tac >>
-                rw [check_ctors_def]) >>
-     metis_tac [],
- metis_tac [],
- induct_on `pes` >>
-     rw [] >>
-     fs [check_ctors_def] >>
-     `?p e. h = (p,e)` by metis_tac [pair_CASES] >>
-     rw [] >>
-     fs [check_ctors_def, LET_THM] >>
-     disj1_tac >>
-     qexists_tac `v` >>
-     qexists_tac `(count',s')` >>
-     rw [] >>
-     pop_assum match_mp_tac >>
-     rw [] >>
-     rw [] >>
-     `?p e. e'' = (p,e)` by metis_tac [pair_CASES] >>
-     rw [] >>
-     fs [EVERY_MEM] >>
-     res_tac >>
-     fs [],
+ metis_tac [check_ctors_result_def, check_ctors_v_def],
+ metis_tac [eval_ctor_inv_lookup, check_ctors_result_def],
+ metis_tac [check_ctors_result_def, check_ctors_v_def],
+ metis_tac [check_ctors_result_def, check_ctors_v_def],
+ metis_tac [check_ctors_result_def, check_ctors_v_def, eval_ctor_inv_def],
+ metis_tac [check_ctors_result_def, eval_ctor_inv_do_uapp],
+ metis_tac [check_ctors_result_def, check_ctors_v_def],
+ metis_tac [check_ctors_result_def, check_ctors_v_def],
+ `check_ctors cenv e'' ∧
+  eval_ctor_inv cenv s'' env'`
+        by prove_tac [eval_ctor_inv_do_app] >>
+     rw [] >|
+     [fs [eval_ctor_inv_def] >>
+          metis_tac [],
+      metis_tac []],
+ metis_tac [check_ctors_result_def, check_ctors_v_def],
+ metis_tac [check_ctors_result_def, check_ctors_v_def],
+ metis_tac [check_ctors_result_def, check_ctors_v_def],
+ metis_tac [check_ctors_result_def, eval_ctor_inv_do_log],
+ metis_tac [check_ctors_result_def, check_ctors_v_def],
+ metis_tac [check_ctors_result_def, check_ctors_v_def],
+ metis_tac [check_ctors_result_def, eval_ctor_inv_do_if],
+ metis_tac [check_ctors_result_def, check_ctors_v_def],
+ metis_tac [check_ctors_result_def, check_ctors_v_def],
  cases_on `pes` >>
      fs [check_ctors_def] >>
      `?p e. h = (p,e)` by metis_tac [pair_CASES] >>
      rw [] >>
-     fs [check_ctors_def, LET_THM],
- metis_tac [],
- metis_tac [],
- metis_tac [],
- unfinished,
- unfinished,
- unfinished]
+     fs [check_ctors_def, LET_THM, EVERY_MEM, LAMBDA_PROD, GSYM PFORALL_THM,
+         GSYM PEXISTS_THM] >>
+     metis_tac [],
+ cases_on `pes` >>
+     fs [check_ctors_def] >>
+     `?p e. h = (p,e)` by metis_tac [pair_CASES] >>
+     rw [] >>
+     fs [check_ctors_def, LET_THM, EVERY_MEM, LAMBDA_PROD, GSYM PFORALL_THM,
+         GSYM PEXISTS_THM] >>
+     metis_tac [],
+ metis_tac [check_ctors_result_def, check_ctors_v_def, eval_ctor_inv_bind_env],
+ metis_tac [check_ctors_result_def, check_ctors_v_def],
+ `eval_ctor_inv cenv s (build_rec_env funs env env)` 
+            by (rw [build_rec_env_def] >>
+                match_mp_tac eval_ctor_build_rec_env >>
+                fs [eval_ctor_inv_def, EVERY_MEM]) >>
+     rw [] >>
+     fs [eval_ctor_inv_def, EVERY_MEM] >>
+     metis_tac [],
+ metis_tac [check_ctors_result_def, check_ctors_v_def],
+ rw [check_ctors_result2_def],
+ rw [check_ctors_result2_def] >>
+     metis_tac [check_ctors_result2_def, check_ctors_result_def],
+ rw [check_ctors_result2_def] >>
+     metis_tac [check_ctors_result2_def, check_ctors_result_def],
+ metis_tac [check_ctors_result2_def, check_ctors_result_def],
+ metis_tac [check_ctors_result2_def, check_ctors_result_def],
+ `pmatch cenv s p v env = Match env' ∧ eval_ctor_inv cenv s env'` 
+         by metis_tac [pmatch'_pmatch2, match_result_distinct, check_ctors_match_result_def] >>
+     rw [] >>
+     fs [eval_ctor_inv_def] >>
+     metis_tac [],
+ `(pmatch cenv s p v env = No_match) ∨ 
+  ((pmatch cenv s p v env = Match_type_error) ∧
+   ?t1 t2. get_pat_type cenv p = SOME t1 ∧ get_val_type cenv v = SOME t2 ∧ t1 ≠ t2)`
+             by metis_tac [pmatch'_pmatch2, match_result_distinct] >|
+     [`(pes = []) ∨ ?p' e' pes'. pes = (p',e')::pes'` 
+            by (cases_on `pes` >>
+                rw [] >>
+                cases_on `h` >>
+                metis_tac []) >>
+          fs [] >>
+          `get_pat_type cenv p' = get_pat_type cenv p` 
+                    by (rw [] >>
+                        fs [LAMBDA_PROD, GSYM PFORALL_THM] >>
+                        metis_tac [get_pat_type_thm]) >>
+          metis_tac [],
+      `evaluate_match' s env v pes (s,Rerr (Rraise Bind_error)) ∨
+       evaluate_match' s env v pes (s,Rerr Rtype_error)`
+                 by metis_tac [eval'_to_eval2_lem] >>
+          imp_res_tac big_exp_determ' >>
+          fs [check_ctors_result_def]],
+ `pmatch cenv s p v env = Match_type_error` by metis_tac [pmatch'_pmatch2, match_result_distinct] >>
+     rw [check_ctors_result_def],
+ metis_tac [check_ctors_result_def, check_ctors_v_def]]);
 
+val check_ctors_dec_def = Define `
+(check_ctors_dec cenv (Dlet p e) = (check_ctors_p cenv (get_pat_type cenv p) p ∧ check_ctors cenv e)) ∧
+(check_ctors_dec cenv (Dletrec funs) = EVERY (λ(f,x,e). check_ctors cenv e) funs) ∧
+(check_ctors_dec cenv (Dtype _) = T)`;
 
- *) 
+val check_ctors_result3_def = Define `
+(check_ctors_result3 cenv (Rval (cenv',env)) = 
+  EVERY (λ(x,v). check_ctors_v cenv v) env) ∧
+(check_ctors_result3 cenv _ = T)`;
 
+val eval_dec'_to_eval_dec_simple_pat = Q.store_thm ("eval_dec'_to_eval_dec_simple_pat",
+`!mn menv cenv s env d s' r.
+   (r ≠ Rerr (Rraise Bind_error)) ∧
+   check_ctors_dec cenv d ∧ 
+   eval_ctor_inv cenv s env ∧
+   evaluate_dec' mn menv cenv s env d (s',r)
+   ⇒
+   evaluate_dec mn menv cenv s env d (s',r) ∧
+   eval_ctor_inv cenv s' env ∧
+   check_ctors_result3 cenv r`,
+rw [evaluate_dec_cases, evaluate_dec'_cases] >>
+fs [check_ctors_dec_def, check_ctors_result3_def] >|
+[`evaluate F menv cenv (0,s) env e ((0,s'), Rval v) ∧
+  eval_ctor_inv cenv s' env ∧
+  check_ctors_result cenv (Rval v)`
+        by metis_tac [eval'_to_eval_simple_pat, result_distinct] >>
+     fs [check_ctors_result_def] >>
+     `eval_ctor_inv cenv s' (emp:(string,v) env)`
+                 by fs [eval_ctor_inv_def, LibTheory.emp_def] >>
+     metis_tac [pmatch'_pmatch2, match_result_distinct],
+ metis_tac [eval'_to_eval_simple_pat, result_distinct],
+ `evaluate F menv cenv (0,s) env e ((0,s'), Rval v) ∧
+  eval_ctor_inv cenv s' env ∧
+  check_ctors_result cenv (Rval v)`
+        by metis_tac [eval'_to_eval_simple_pat, result_distinct] >>
+     fs [check_ctors_result_def] >>
+     `eval_ctor_inv cenv s' (emp:(string,v) env)`
+                 by fs [eval_ctor_inv_def, LibTheory.emp_def] >>
+     metis_tac [check_ctors_match_result_def, pmatch'_pmatch2, match_result_distinct, eval_ctor_inv_def],
+ `evaluate F menv cenv (0,s) env e ((0,s'), Rval v) ∧
+  eval_ctor_inv cenv s' env ∧
+  check_ctors_result cenv (Rval v)`
+        by metis_tac [eval'_to_eval_simple_pat, result_distinct] >>
+     fs [check_ctors_result_def] >>
+     `eval_ctor_inv cenv s' (emp:(string,v) env)`
+                 by fs [eval_ctor_inv_def, LibTheory.emp_def] >>
+     metis_tac [check_ctors_match_result_def, pmatch'_pmatch2, match_result_distinct, eval_ctor_inv_def],
+ metis_tac [eval'_to_eval_simple_pat, result_distinct],
+ metis_tac [eval'_to_eval_simple_pat, result_distinct, error_result_distinct, result_11],
+ metis_tac [eval'_to_eval_simple_pat, result_distinct, error_result_distinct, result_11],
+ fs [LibTheory.emp_def, eval_ctor_inv_def] >>
+     metis_tac [SIMP_RULE (srw_ss()) [eval_ctor_inv_def] eval_ctor_build_rec_env, EVERY_DEF,
+                build_rec_env_def],
+ fs [LibTheory.emp_def]]);
 
+ (*
+val check_ctors_result4_def = Define `
+(check_ctors_result4 cenv (Rval env) = 
+  EVERY (λ(x,v). check_ctors_v cenv v) env) ∧
+(check_ctors_result4 cenv _ = T)`;
+
+val eval_decs'_to_eval_decs_simple_pat = Q.store_thm ("eval_decs'_to_eval_decs_simple_pat",
+`!mn menv cenv s env ds s' r cenv'.
+   (r ≠ Rerr (Rraise Bind_error)) ∧
+   EVERY (check_ctors_dec cenv) ds ∧ 
+   eval_ctor_inv cenv s env ∧
+   evaluate_decs' mn menv cenv s env ds (s',cenv',r)
+   ⇒
+   evaluate_decs mn menv cenv s env ds (s',cenv',r) ∧
+   eval_ctor_inv (cenv'++cenv) s' env ∧
+   check_ctors_result4 (cenv'++cenv) r`,
+induct_on `ds` >>
+REPEAT GEN_TAC >>
+rw [Once evaluate_decs_cases, Once evaluate_decs'_cases, LibTheory.emp_def,
+    check_ctors_result4_def] >>
+rw [check_ctors_result4_def] >-
+metis_tac [eval_dec'_to_eval_dec_simple_pat, result_distinct, error_result_distinct, result_11] >-
+ metis_tac [eval_dec'_to_eval_dec_simple_pat, result_distinct, error_result_distinct, result_11] >>
+`evaluate_dec mn menv cenv s env h (s2,(Rval (new_tds,new_env))) ∧
+ eval_ctor_inv cenv s2 env ∧ 
+ check_ctors_result3 cenv (Rval (new_tds,new_env))`
+       by metis_tac [eval_dec'_to_eval_dec_simple_pat, result_distinct, error_result_distinct, result_11] >>
+fs [LibTheory.merge_def, check_ctors_result3_def] >>
+`eval_ctor_inv (new_tds ++ cenv) s2 (new_env++env)` by cheat >>
+`EVERY (check_ctors_dec (new_tds ++ cenv)) ds` by cheat >>
+`evaluate_decs mn menv (new_tds ++ cenv) s2 (new_env ++ env) ds (s',new_tds',r') ∧
+ eval_ctor_inv (new_tds' ++ new_tds ++ cenv) s' (new_env ++ env) ∧
+ check_ctors_result4 (new_tds' ++ new_tds ++ cenv) r'`
+       by (cases_on `r'` >>
+           fs [combine_dec_result_def] >>
+           metis_tac [APPEND_ASSOC, result_distinct, error_result_distinct, result_11]) >-
+metis_tac [] >-
+fs [eval_ctor_inv_def] >>
+cases_on `r'` >>
+fs [combine_dec_result_def, check_ctors_result4_def, LibTheory.merge_def, eval_ctor_inv_def]);
+
+val check_ctors_top_def = Define `
+(check_ctors_top cenv (Tdec d) =
+  check_ctors_dec cenv d) ∧
+(check_ctors_top cenv (Tmod mn specs ds)  =
+  EVERY (check_ctors_dec cenv) ds)`;
+
+val check_ctors_result5_def = Define `
+(check_ctors_result5 cenv (Rval (menv,env)) = 
+  EVERY (λ(x,v). check_ctors_v cenv v) env) ∧
+(check_ctors_result5 cenv _ = T)`;
+
+val eval_top'_to_eval_top_simple_pat = Q.store_thm ("eval_top'_to_eval_top_simple_pat",
+`!menv cenv s env top s' cenv' r.
+   (r ≠ Rerr (Rraise Bind_error)) ∧
+   check_ctors_top cenv top ∧ 
+   eval_ctor_inv cenv s env ∧
+   evaluate_top' menv cenv s env top (s',cenv',r)
+   ⇒
+   evaluate_top menv cenv s env top (s',cenv',r) ∧
+   eval_ctor_inv (cenv'++cenv) s' env ∧
+   check_ctors_result5 (cenv'++cenv) r`,
+
+rw [evaluate_top_cases, evaluate_top'_cases] >>
+fs [check_ctors_top_def, check_ctors_result5_def] >>
+
+metis_tac [eval_decs'_to_eval_decs_simple_pat, eval_dec'_to_eval_dec_simple_pat, 
+           eval_ctor_inv_def, result_distinct, error_result_distinct, result_11] >>
+
+           *)
+      
 val _ = export_theory ();
